\nopagenumbers
{\bf Theorem: Sum of the First $n$ Integers}
\vskip 1mm
\hrule

\vskip 6pt
For all intgers $n\geq 1$ $$1+2+\cdots+n={n(n+1)\over 2}$$

\vskip 10pt
{\bf Proof (by mathematical induction)}

\vskip 6pt
Let the property $P(n)$ be the equation 

$$1+2+\cdots+n={n(n+1)\over 2} \qquad\hbox{$\longleftarrow P(n)$}\qquad$$

{\bf Show that $P(1)$ is true}:

\vskip 1mm
To establish $P(1)$, we must show that

$$1={1(1+1)\over 2} \qquad\hbox{$\longleftarrow P(1)$}\qquad$$

But the left-hand side of the equation is $1$ and the right-hand side is

$$1={1(1+1)\over 2}={2\over 2}=1$$

also. Hence $P(1)$ is true.

\vskip 6pt
{\bf Show that for all integers $k\geq 1$, if $P(k)$ is true then $P(k+1)$ is also true}:

\vskip 1mm
[Suppose that $P(k)$ is true for a particular but arbitrarily chosen integer $k\geq 1$. That is:] Suppose that $k$ is any integer with $k\geq 1$ such that

$$1+2+3+\cdots+k={k(k+1)\over 2}\qquad\hbox{$\longleftarrow P(k)$ inductive hypothesis}\qquad$$

[We must show that $P(k+1)$ is true, That is:] We must show that

$$1+2+3+\cdots+(k+1)={(k+1)[(k+1)+1]\over 2}$$

or, equivalently, that

$$1+2+3+\cdots+(k+1)={(k+1)[(k+2)]\over 2}$$

[We will show that the left-hand side and the right-hand side of $P(k+1)$ are equal to the same quantity and thus are equal to each other.]

\vskip 1mm
The left-hand side of $P(k+1)$ is

$$\eqalign{1+2+3+\cdots+(k+1)&= 1+2+3+\cdots+k+(k+1)\qquad\hbox{making the next-to-last term explict}\cr
			&={{k+(k+1)\over 2}+(k+1)}\cr
			&={{k+(k+1)\over 2}+{2(k+1)\over 2}}\cr
			&= {{k^2+k}\over 2}+{2(k+1)\over 2}\cr
			&= {{k^2+3k+2}\over 2}\cr}$$

And the right-hand side of $P(k+1)$ is $${{{(k+1)(k+2)}\over 2}={{k^2+3k+2}\over 2}}$$



\vfill\eject
