\nopagenumbers
{\bf Example 1:} Solve the differential equation

$${dy\over dx}={2xy^2+1\over 2x^2y}$$

\vskip 10pt
{\bf Solution}

\vskip 6pt
Some of the choices of differential forms corresponding to this equation are

$$\eqalign{(2xy^2+1)dx+2x^2y\,dy&=0\cr
	{2xy^2+1\over 2x^y}dx+dy&=0\cr
	dx+{2x^2y\over 2xy^2+1}dy&=0\cr}$$

However, the firt form is best for our purposes because it is a total differential of the function $F(x,y)=x^2y^2+x$:

$$\eqalign{(2xy^2+1)dx+2x^2y\,dy&=d\bigl[x^2y^2+x\bigr]\cr
	&={\partial\over\partial x}(x^2y^2+x)dx+{\partial\over\partial y}(x^2y^2+x)dy\cr}$$

Thus, the solutions are given implicitly by the formula $x^2y^2+x=C$

\vfill\eject
\bye
