\nopagenumbers
{\bf Theorem: Alternating Series Test}
\vskip 6pt
Let $a_n>0$. The alternating series $$\sum_{n=1}^\infty(-1)^na_n \;\; and \;\; \sum_{n=1}^\infty(-1)^{n+1}a_n$$ converge when these two conditions are met.
\vskip 1mm
$1.$ $\lim_{n\to\infty} a_n=0$ 
\vskip 1mm
$2.$ $a_{n+1} \leq a_n$ for all $n$
\vskip 10pt
{\bf Proof:}
\vskip 6pt
Consider the alternating series $$\sum_{n=1}^\infty(-1)^{n+1}a_n$$ For this series, the partial sum $$S_{2n}=(a_1-a_1)+(a_3-a_4)+(a_5-a_6)+\ldots+(a_{2n-1}-a_{2n})$$ has all non-negative terms, and therefore $(S_{2n})$ is a non-decreasing sequence. But you can also write $$S_{2n}=a_1-(a_2-a_3)-(a_4-a_5)-\ldots-(a_{2n-2}-a_{2n-1})-a_{2n}$$ which implies that $S_{2n} \leq a_1$ for every integer $n$. So $(S_{2n})$ is a bounded, non-decreasing sequence that converges to some value $L$. Because $S_{2n-1}-a_{2n}=S_{2n}$ and $a_{2n}\to 0$, you have $$\lim_{n\to\infty} S_{2n-1}=\lim_{n\to\infty}S_{2n}+\lim_{n\to\infty}a_{2n}$$ $$=L+\lim_{n\to\infty}a_{2n}$$ $$=L$$ Because both $S_{2n}$ and $S_{2n-1}$ converge to the same limit $L$, it follows that $(S_n)$ also converges to $L$. Consequently, the given alternating series converges.


\vfill\eject
