\nopagenumbers
{\bf Example 3:} For the initial value problem

$$y'+y=\sqrt{1+\cos^2(x)},\quad y(1)=4$$

find the value of $y(2)$

\vskip 10pt
{\bf Solution}

\vskip 6pt
The intergrating factor for the differential equation is, from $\mu(x)=e^{\int P(x)\,dx}$

$$\mu(x)=e^{\int 1dx}=e^x$$

The general solution from $y(x)={1\over\mu(x)\Bigl[\int\mu(x)Q(x)dx+C\Bigr]}$ thus reads

\vskip 3mm
$$y(x)=e^{-x}\Bigl(\int e^x\sqrt{1+\cos^2(x)}dx+C\Bigr)$$

and take the definite integral from the initial value $x=1$ to the desired value $x=2$:

$$e^xy\bigg\vert^{x=2}_{x=1}=e^2y(2)-e^1y(1)=\int^{x=2}_{x=1}e^x\sqrt{1+\cos^2(x)}dx$$

Inserting the given value of $y(1)$ and solving, we express

$$y(2)=e^{-2+1}(4)+e^{-2}\int^2_1e^x\sqrt{1+\cos^2(x)}dx$$

Using Simpson's Rule, we find that the definite integral is approximately $4.841$, so

$$y(2)\approx 4e^{-1}+4.841e^{-2}\approx 2.127$$

\vfill\eject
\bye
