\nopagenumbers
{\bf Example 7:} As shown in Example 2, the function $\phi(x)=c_1e^{-x}+c_2e^{2x}$ is a solution to

$${d^2y\over dx^2}-{dy\over dx}-2y=0$$

for any choice of the constants $c_1$ and $c_2$. Determine $c_1$ and $c_2$ so that the initial conditions

$$y(0)=2\quad\hbox{and}\quad {dy\over dx}(0)=-3$$

are satisfied.


\vskip 10pt
{\bf Solution}

\vskip 6pt
To determine the constants $c_1$ and $c_2$, we first compute $d\phi\over dx$ to get ${d\phi\over dx}=-c_1e^{-x}+2c_2e^{2x}$. Substituting in our initial conditions gives the following systems of equations:

$$\cases{\eqalign{\phi(0)&=c_1e^0+c_2e^0=2\cr
	{d\phi\over dx}(0)&=-c_1e^0+2c_2e^0=-3}}\quad\hbox{or}\quad\cases{\eqalign{c_1+c_2&=2\cr
									-c_1+2c_2&=-3}}$$

Adding the last two equations yields $3c_2=-1$, so $c_2=-{1\over 3}$. Since $c_1+c_2=2$, we find $c_1={7\over 3}$. Hence, the solution to the initial value problem is $\phi(x)=({7\over 3})e^{-x}-({1\over 3})e^{2x}$.



\vfill\eject
\bye
