\nopagenumbers
{\bf Theorem: 1.4-1}
\vskip 1mm
\hrule

\vskip 6pt
If $A$ and $B$ are independent events, then the followin pairs of events are also independent:

\vskip 6pt
(a) $A$ and $B'$

\vskip 6pt
(b) $A'$ and $B$

\vskip 6pt
(c) $A'$ and $B'$

\vskip 10pt
{\bf Proof}

\vskip 6pt
We know that conditional probability satisfies the axioms for a probability function. Hence, if $P(A)>0$, then $P(B'|A)=1-P(B|A)$. Thus

$$\eqalign{P(A\cap B')&=P(A)P(B'|A)=P(A)\bigl[1-P(B|A)\bigr]\cr
		&=P(A)\bigl[1-P(B)\bigr]\cr
		&=P(A)P(B')\cr}$$

because $P(B|A)=P(B)$ by hypothesis. If $P(A)=0$, then $P(A\cap B')=0$, so in this case we also have $P(A\cap B')=P(A)P(B')$. Consequently, $A$ and $B'$ are independent events.

\vfill\eject
\bye
