\nopagenumbers
{\bf Example 4}: Solve

$$(-3x+y+6)dx+(x+y+2)dy=0$$

{\bf Solution}

\vskip 6pt
Since $a_1b_2=(-3)(1)\neq(1)(1)=a_2b_1$, we will use the translation of axes $x=u+h, y=v+k$, where $h$ and $k$ satisfy the system

$$\eqalign{-3h+k+6&=0\cr
	h+k+2&=0\cr}$$

Solving the above system for $h$ and $k$ gives $h=1,k=-3$. Hence, we let $x=u+1$ and $y=v-3$. Because $dy=dv$ and $dx=du$, substituting in $(-3x+y+6)dx+(x+y+2)dy=0$ for $x$ and $y$ yields

$$\eqalign{(-3u+v)du+(u+v)dv&=0\cr
	{dv\over du}&={3-\Bigl({u\over v}\Bigr)}\over 1+\Bigl({v\over u}\Bigr)\cr}$$

The last equation is homogeneous, so we let $z={v\over u}$. Then ${dv\over du}=z+u(dz\over du)$, and substituting for ${v\over u}$, we obtain

$$z+u{dz\over du}={3-z\over 1+z}$$

Separating variables gives

$$\eqalign{\int{z+1\over z^2+2z-3}dz&=-\int{1\over u}du\cr
	{1\over 2}\ln|z^2+2z-3|&=-\ln|u|+C_1\cr}$$

for which it follows that

$$z^2+2z-3=Cu^{-2}$$

When we substitute back in for $z,u$, and $v$, we find

$$\eqalign{\Bigl({v\over u}\Bigr)^2+2\Bigl({v\over u}\Bigr)-3&=Cu^{-2}\cr
		v^2+2uv-3u^2&=C\cr
		(y+3)^2+2(x-1)(y+3)-3(x-1)^2&=C\cr}$$

This last equation gives an implicit solution to $(-3x+y+6)dx+(x+y+2)dy=0$

\vfill\eject
\bye
