\nopagenumbers
{\bf Example 4:} Show that

$$x+y+e^{xy}=0$$

is an implicit solution to the nonlinear equation

$$\bigl(1+xe^{xy}\bigr){dy\over dx}+1+ye^{xy}=0$$

\vskip 10pt
{\bf Solution}

\vskip 6pt
First, we observe that we are unable to solve $x+y+e^{xy}=0$ directly for $y$ in terms of $x$ alone. However, for $x+y+e^{xy}=0$ to hold, we realize that any change in $x$ requires a change in $y$,so we expect the relation $x+y+e^{xy}=0$ to define implicitly at least one function $y(x)$. This is difficult to show directly but can be rigorously verified using the {\bf implicit function theorem} of advanced calculus, which guarantes that such a function $y(x)$ exists that is also differentiable.

\vskip 1mm
Once we know that $y$ is a differentiable function of $x$, we can use te technique of implicit differentiation. Indeed, from $x+y+e^{xy}=0$ we obtain on differentiating with respect to $x$ and applying the product and chain rules,

$${d\over dx}(x+y+e^{xy})=1+{dy\over dx}+e^{xy}\Biggl(y+x{dy\over dx}\Biggr)=0$$

or

$$(1+xe^{xy}){dy\over dx}+1+ye^{xy}=0$$

which is identical to the differential equation $\bigl(1+xe^{xy}\bigr){dy\over dx}+1+ye^{xy}=0$. Thus, relation $x+y+e^{xy}=0$ is an implicit solution on some interval guaranteed by the implicit function theorem.

\vfill\eject
\bye
