\nopagenumbers
{\bf Example 2}:  Solve

$$(2xy-\sec^2(x))dx+(x^2+2y)dy=0$$

\vskip 10pt
{\bf Solution}

\vskip 6pt
Here $M(x,y)=2xy-\sec^2(x)$ and $N(x,y)=x^2+2y$. Because

$${\partial M\over\partial y}=2x={\partial N\over\partial x}$$

$(2xy-\sec^2(x))dx+(x^2+2y)dy=0$ is exact. To find $F(x,y)$, we begin by intergrating $M$ with respect to $x$:

$$\eqalign{F(x,y)&=\int(2xy-\sec^2(x))dx+g(y)\cr
	&=x^2y-\tan(x)+g(y)\cr}$$

Next we take the partial derivative of $F(x,y)=\int(2xy-\sec^2(x))dx+g(y)$ with respect to $y$ and substitute $x^2+2y$ for $N$:

$$\eqalign{{\partial F\over\partial y}(x,y)&=N(x,y)\cr
	x^2+g'(y)&=x^2+2y\cr}$$

Thus $g'(y)=2y$, and since the choice of the constant of integration is not important, we can take $g'(y)=y^2$. Hence from $F(x,y)=\int(2xy-\sec^2(x))dx+g(y)$, we have $x^2y-\tan(x)+y^2$, and the solution to $(2xy-\sec^2(x))dx+(x^2+2y)dy=0$  is given implicitly by $x^2y-\tan(x)+y^2=C$

\vfill\eject
\bye
