\nopagenumbers
{\bf Example 4}: Show that

$$\Bigl(x+3x^3\sin(y)\Bigr)dx+\Bigl(x^4\cos(y)\Bigr)=0$$

is {\it not} exact but that multiplying this equation by the factor $x^{-1}$ yields an exact equation. Use this fact to solve $\Bigl(x+3x^3\sin(y)\Bigr)dx+\Bigl(x^4\cos(y)\Bigr)=0$

\vskip 10pt
{\bf Solution}

\vskip 6pt
In $\Bigl(x+3x^3\sin(y)\Bigr)dx+\Bigl(x^4\cos(y)\Bigr)=0$, $M=x+3x^3\sin(y)$ and $N=x^4\cos(y)$. Because

$${\partial M\over\partial y}=3x^3\cos(y)\neq 4x^3\cos(y)={\partial N\over\partial x}$$

$\Bigl(x+3x^3\sin(y)\Bigr)dx+\Bigl(x^4\cos(y)\Bigr)=0$ is not exact. When we multiply $\Bigl(x+3x^3\sin(y)\Bigr)dx+\Bigl(x^4\cos(y)\Bigr)=0$ by the factor $x^{-1}$, we obtain

$$\Bigl(1+3x^2\sin(y)\Bigr)dx+\Bigl(x^3\cos(y)\Bigr)dy=0$$

For this new equation, $M=1+3x^2\sin(y)$ and $N=x^3\cos(y)$. If we test for exactness, we now find that

$${\partial M\over\partial y}=3x^2\cos(y)={\partial N\over\partial x}$$

and hence $\Bigl(1+3x^2\sin(y)\Bigr)dx+\Bigl(x^3\cos(y)\Bigr)dy=0$ is exact. Upon solving $\Bigl(1+3x^2\sin(y)\Bigr)dx+\Bigl(x^3\cos(y)\Bigr)dy=0$, we find that the solution is given implicitly by $x+x^3\sin(y)=C$. Since equations $\Bigl(x+3x^3\sin(y)\Bigr)dx+\Bigl(x^4\cos(y)\Bigr)=0$ is given implicitly by $x+x^3\sin(y)=C$.

\vfill\eject
\bye
