\nopagenumbers
{\bf Example 1:} Find the general solution to

$${1\over x}{dy\over dx}-{2y\over x^2}=x\cos(x),\quad x>0$$

\vskip 10pt
{\bf Solution}

\vskip 6pt
To put this linear equation in standard form, we multiply by $x$ to obtain

$${dy\over dx}-{2\over x}y=x^2\cos(x)$$

Here $P(x)={-2\over x}$, so

$$\int P(x)dx=\int{-2\over x}dx=-2\ln|x|$$

Thus, an integrating factor is

$$\mu(x)=e^{-2\ln|x|}=e^{\ln(x^{-2})}=x^{-2}$$

Multiplying $${dy\over dx}-{2\over x}y=x^2\cos(x)$$ by $\mu(x)$ yields

$$\eqalign{\underbrace{x^{-2}{dy\over dx}-2x^{-3}y}&=\cos(x)\cr
		{d\over dx}(x^{-2}y)&=\cos(x)\cr}$$

We now integrate both sides and solve for $y$ to find

$$\eqalign{x^{-2}y&=\int\cos(x)dx=\sin(x)+C\cr
	y&=x^2\sin(x)+Cx^2}$$

It is easily checked yhat this solution is valid for all $x>0$

\vfill\eject
\bye
