\nopagenumbers
{\bf Example 3}: Solve

$${dy\over dx}-5y=-{5\over 2}xy^3$$

\vskip 6pt
{\bf Solution}
This is a Bernoulli equation with $n=3,P(x)=-5$ and $Q(x)=-{5\over 2}$. To transform ${dy\over dx}-5y=-{5\over 2}xy^3$ into a linear equation, we first divide by $y^3$ to obtain

$$y^{-3}{dy\over dx}-5y^{-2}=-{5\over 2}x$$

Next we make the substitution $v=y^{-2}$. Since ${dv\over dx}=-2y^{-3}{dy\over dx}$, the transformed equation is

$$\eqalign{-{1\over 2}{dv\over dx}-5v&=-{5\over 2}x\cr
		{dv\over dx}+10v&=5x\cr}$$

${dv\over dx}+10v=5x$ is linear, so we can solve it for $v$. It turns out

$$v={x\over 2}-{1\over 20 +Ce^{-1x}}$$

Not included in the last equation is the solution $y\equiv 0$ that was lost in the process of ${dy\over dx}-5y=-{5\over 2}xy^3$ by $y^3$
\vfill\eject
\bye
