\nopagenumbers
{\bf Example 2:} Show that for {\it any} choice of the constants $c_1$ and $c_2$, the function

$$\phi(x)=c_1e^{-x}+c_2e^{2x}$$

is an explicit solution to the linear equation

$$y''-y'-2y=0$$

\vskip 10pt
{\bf Solution}

\vskip 6pt
We compute $\phi(x)=-c_1e^{-x}+2c_2e^{2x}$ and $\phi''(x)=c_1e^{-x}+4c_2e^{2x}$. Substitution of $\phi,\phi'$ and $\phi''$ for $y,y'$ and $y''$ in the equation yields

$$\bigl(c_1e^{-x}+4c_2e^{2x}\bigr)-\bigl(c_1e^{-x}+2c_2e^{2x}\bigr)-2\bigl(c_1e^{-x}+c_2e^{2x}\bigr)=\bigl(c_1+c_1-2c_1\bigr)e^{-x}+\bigl(4c_2-2c_2-2c_2\bigr)e^{2x}=0$$

Since equality holds for all $x$ in $(-\infty,\infty)$, then $\phi(x)=c_1e^{-x}+c_2e^{2x}$ is an explicit solution to the equation on the interval $(-\infty,\infty)$ for any choice of the constants $c_1$ and $c_2$

\vfill\eject
\bye
