\nopagenumbers
{\bf Definition: Recursive Definitions of sum and Product}
\vskip 1mm
\hrule

\vskip 6pt
Given numbers $a_1,a_2,\ldots ,a_n$, where $n$ is a positive integer, the {\bf summation from $i=1$ to $n$ of the $a_i$, denoted $\sum^n_{i=1}a_i$, is defined as}:

$$\sum^1_{i=1}a_i=a_1 \quad\hbox{and} \quad \sum^n_{i=1}a_i=\Biggl(\sum^{n-1}_{i=1}a_i \Biggr)+ a_n, \qquad\hbox{if $n>1$}$$

The {\bf product from $i=1$ to $n$ of the $a_i$, denoted $\prod^n_{i=1}a_i$, is defined by}

$$\prod^1_{i=1}a_i=a_1 \quad\hbox{and} \quad \prod^n_{i=1}a_i=\Biggl(\prod^{n-1}_{i=1}a_i \Biggr)\cdot a_n, \qquad\hbox{if $n>1$}$$

\vfill\eject
\bye
