\nopagenumbers
{\bf Theorem: Limit of the $n^{th}$ Term of a Convergent Series}
\vskip 6pt
If $\sum_{n=1}^\infty a_n$ converges, then $\lim_{n\to\infty}a_n=0$.
\vskip 10pt
{\bf Proof:}
\vskip 6pt
Assume that $$\sum_{n=1}^\infty a_n=\lim_{n\to\infty}S_n=L$$ Then, because $$S_n=S_{n-1}+a_n$$ and $$\lim_{n\to\infty}S_n=\lim_{n\to\infty}S_{n-1}=L$$ it follows that $$L=\lim_{n\to\infty}S_n$$ $$=\lim_{n\to\infty} (S_{n-1}+a_n)$$ $$=\lim_{n\to\infty} S_{n-1}+\lim_{n\to\infty}a_n$$ $$=L+\lim_{n\to\infty}a_n$$ which implies that $(a_n)$ converges to $0$.

\vfill\eject
