Name: {\bf Jordan Suber}

\centerline {Mid-Term 2}
\vskip 2pc

$(1a)$ The symbol $\sum a_n$ means the sequence of numbers.
\vskip 1pc

$(1b)$ The expression $\sum^\infty_{n=1}a_n$ is a number and the limit $$\lim_{n\to\infty}\sum^n_{i=1}a_j$$
\vskip 1pc

$(1c)$ We say$\sum a_n$ is {\bf convergent} if the limit exists and is finite.

\vskip 2pc

$(2)$ {\bf nth term criterion for Divergence}
\vskip 6pt
{\bf Definitions}
\vskip 1pt

$(S_n)$ --- $n^{th}$ partial sum
\vskip 1pt

$L$ --- The limit of a sequence $(a_n)$. $L$ is a real number $\{ L \in \Re\}$
\vskip 1pt

$(a_n)$ --- A sequence of real numbers
\vskip 6pt

{\bf Proof}
\vskip 1pt
$$\lim_{n\to\infty}=0$$
\vskip 1pt
Assume that $\sum^\infty_{n=1}a_n=\lim_{n\to\infty}S_n=L$. The $n^{th}$ term in a recursively defined sequence is equal to $$S_n=S_{n-1}+a_n$$ \centerline {and} $$\lim_{n\to\infty}S_n=\lim_{n\to\infty}S_{n-1}=L$$ it follows that $$\eqalign{L&=\lim_{n\to\infty}S_n\cr
				&=\lim_{n\to\infty}(S_{n-1}+a_n)\cr
				&=\lim_{n\to\infty}S_{n-1}+\lim_{n\to\infty}a_n\cr
				&=L+\lim_{n\to\infty}a_n}$$
Which implies that $(a_n)$ converges to $0$.
\vskip 2pc

$(3a)$ $a_n$ {\bf converges}.
\vskip 1pt

$(3b)$ No conclusion can be made about $b_n$.
\vskip 1pt

$(3c)$ No conclusion can be made about $a_n$.
\vskip 1pt

$(3d)$ $b_n$ {\bf diverges}.
\vskip 1.5in

$(5a)$ $$\eqalign{	\lim_{n\to\infty}{n^2+2\over n^4-4n^3}&=0\cr
			\lim_{n\to\infty}{{n^2/n^4+2/n^4}\over{n^4/n^4-4n^3/n^4}}	&=lim_{n\to\infty}{{1/n^2+2/n^4}\over{1-4n/n}}\cr
											&={0+0\over 1-0}\cr
											&={0\over 1}\cr
											&=0\cr}$$
\vskip 1pc
$(5b)$ $$\eqalign{	\lim_{n\to\infty}{n^2\over 3^n}&=0\cr
			\lim_{n\to\infty}{{{(n+1)}^2/ 3^{n+1}}\over {n^2/ 3^n}}  &= \lim_{n\to\infty}{{{(n+1)}^2 3^n\over 3^{n+1}{n^2}}}\cr
									&= \lim_{n\to\infty}{(n+1)^2\over 3n^2} \cr
									&= {1\over 3}\cr}$$
\vskip 1pt
$\lim_{n\to\infty}{n^2\over 3^n}$ converges to $1\over 3$.

\vskip 1pc
$(5c)$ $$\eqalign{	\lim_{n\to\infty}{ {3^n} {((n))}^2\over {(2n)!}} &= {\lim_{n\to\infty}{ {3^{n+1}} {(({n+1}))}^2 / {(2({n})!} \over {3^n} {((n))}^2/ {(2({n+1})!} }}\cr
									&=	\lim_{n\to\infty}{ {3^{n+1}} {(({n+1})!)}^2 {(2n)!}\over {3^n} {((n))}^2 {2({n+1})!} }\cr
	  								&=	\lim_{n\to\infty}{ {3{(n+1)}{(n+1)}} \over 2{(n+1)}{(n+1)} }\cr
									&= {{3\over 2} > 1}\cr}$$

\vskip 1pt
The limit of $\lim_{n\to\infty}{ {3^n} {((n))}^2\over {(2n)!}}$, diverges

\vskip 1pc
$(5d)$ From the conclusion of above equation we can make the conclusion that  $$\lim_{n\to\infty}{ {4^n} {((n))}^2\over {(2n)!}}$$ diverges, We use the direct comparision test.

\vskip 1mm
$(6)$ $$\eqalign{	{x^n\over n!} &=   {{x^{(n+1)}/ {(n+1)}!} \over {x^n/ n!}}   \cr
					&= {x\over {n+1} } \cr
					&= {x\over \infty}\cr
					&= {0<1} \cr} $$
\vskip 1mm
Interval of convergence  is $$-\infty < x < \infty$$

\vskip 1mm
$(8a)$ 
$$ {{x^n}\over {n!}} =1+{{x^1}\over {1!}}+{{x^2}\over {2!}}+{{x^3}\over {3!}}+\cdots $$
\vskip 1mm
$f(0)=1$

\vskip 2pc
$(8b)$  $$\eqalign{ f'(x)	&={d\over dx}{\Bigl(1+{{x^1}\over {1!}}+{{x^2}\over {2!}}+{{x^3}\over {3!}}+\cdots\Bigr)}\cr	
				&={0+{{1x^0}\over {1!}}+{{2x^1}\over {2!}}+{{3x^2}\over {3!} }+\cdots}		\cr
				&= 1+{{x^1}\over {1!}}+{{x^2}\over {2!}}+{{x^3}\over {3!}}+\cdots\cr
				&= f(x)\cr}$$


\vfill\eject
