\nopagenumbers
{\bf Theorem: The Inverse of a Product}
\vskip 1mm
\hrule

\vskip 6pt
If $A$ and $B$ are invertible matrices of order $n$, then $AB$ is invertible and

$$(AB)^{-1}=B^{-1}A^{-1}$$

\vskip 10pt
{\bf Proof}

\vskip 6pt
To show that $B^{-1}A^{-1}$ is the inverse of $AB$, you need only show that it conforms to the definition of an inverse matrix. That is,

$$(AB)(B^{-1}A^{-1})=A(BB^{-1})A^{-1}=A(I)A^{-1}=(AI)A^{-1}=AA^{-1}=I$$

In a similar way, $B^{-1}A^{-1})(AB)=I$. So, $AB$ is invertible and its inverse is $B^{-1}A^{-1}$.


\vfill\eject
\bye
